src/riscv/Platform/Run.v
@@ -25,7 +25,7 @@ Section Riscv.
     pc <- getPC;
   inst <- loadWord Fetch pc;
   let inst' := decode iset (combine 4 inst) in
-  leakage_event <- leakage_of_instr getRegister inst';
+  leakage_event <- leakage_of_instr regToZ_unsigned regToZ_signed getRegister inst';
   leakEvent leakage_event;;
   execute inst';;
   endCycleNormal.
